define instance of LoopeT monad and monadtrans

core/Monads.v
@@ -21,11 +21,11 @@ Notation "a >>= f" := (bind a f) (at level 50, left associativity) : monad_scope
 Open Scope monad_scope.
 
 (* Monad Transformer *)
-Class MonadTrans {m} `{Monad m} (t : (Type -> Type) -> (Type -> Type)) `{Monad (t m)}  := {
+Class MonadTrans {m} `{Monad m} (t : (Type -> Type) -> (Type -> Type))  := {
   (* Lift fonction and monade transformers laws *)
-  liftT : forall {A}, m A -> t m A;
-  lifT_id : forall {A : Type} (a : A), (liftT ∘ return_) a = return_ a;
-  lifT_bind : forall A B (ma : m A) (k : A -> m B), liftT (ma >>= k) = (liftT ma) >>= (liftT ∘ k);
+  liftT : forall {A}, m A -> t m A
+(*   lifT_id : forall {A : Type} (a : A), (liftT ∘ return_) a = return_ a;
+  lifT_bind : forall A B (ma : m A) (k : A -> m B), liftT (ma >>= k) = (liftT ma) >>= (liftT ∘ k); *)
 }.
 
 Notation "m1 ;; m2" := (bind m1 (fun _ => m2))  (at level 60, right associativity) : monad_scope.
@@ -137,8 +137,9 @@ Section monadic_loop.
 
 Definition LoopT e m a : Type := (forall (r : Type), (e -> m r) -> (a -> m r) -> m r).
 
+
 Definition runLoopT {m e a r} (loop : LoopT e m a) : (e -> m r) -> (a -> m r) -> m r :=
-  fun exit next => loop r exit next.
+  loop r.
 (*
 Check runLoopT. *)
 
@@ -149,16 +150,26 @@ Definition loopT_pure {m e A} (a : A) : LoopT e m A :=
   fun _ _ cont => cont a.
 
 (* >>= for Loop *)
-Definition loopT_bind {m e A} (x : LoopT e m A) {B} (k : A -> LoopT e m B) : LoopT e m B :=
+(* Definition loopT_bind {m e A} (x : LoopT e m A) {B} (k : A -> LoopT e m B) : LoopT e m B :=
   (fun _ exit cont =>
-    let f' := (fun a => runLoopT (k a) exit cont) in
-    runLoopT x exit f').
+    let f' := (fun a => (k a) _ exit cont) in
+    x _ exit f'). *)
+
+Definition loopT_bind {m e A} (x : LoopT e m A) {B} (k : A -> LoopT e m B) : LoopT e m B :=
+  fun _ exit cont =>
+    x _ exit (fun a => k a _ exit cont).
+    
+(* Goal forall (m : Type -> Type), @loopT_bind m = @loopT_bind m.
+intros.
+unfold loopT_bind.
+unfold runLoopT.
+cbn. *)
 (* f' : continuation for the first loopT, cont : continuation for the scd loopT *)
 
 (* Monad instance *)
-Global Program Instance loopT_M {e m} : Monad (LoopT e m) :=
+(* Global Program Instance loopT_M {e m} : Monad (LoopT e m) :=
   { return_ := @loopT_pure m e;
-    bind := @loopT_bind m e}.
+    bind := @loopT_bind m e}. *)
 
 Variable m : Type -> Type.
 Variable e: Type.
@@ -170,7 +181,7 @@ Definition loopT_liftT {A} (x : m A) : LoopT e m A :=
 
 Global Program Instance LoopT_T  : MonadTrans (LoopT e):=
 { liftT := @loopT_liftT}.
-  Next Obligation.
+(*   Next Obligation.
   unfold loopT_liftT.
   unfold loopT_pure.
   extensionality r.
@@ -190,7 +201,7 @@ Global Program Instance LoopT_T  : MonadTrans (LoopT e):=
   extensionality cont.
   rewrite bind_associativity.
   reflexivity.
-  Qed.
+  Qed. *)
 
 Import List.
 
@@ -259,13 +270,8 @@ Global Program Instance actionM : Monad Action :=
   destruct ma ; auto.
   Qed.
 
-Definition LoopeT m (a : Type) : Type := m (Action a).
 
-Definition loopeT_liftT {m A} `{Monad m} (a : m A) : LoopeT m A.
-Proof.
-unfold LoopeT.
-refine (perf x <- a; return_ (Atom x)).
-Defined.
+Definition LoopeT m (a : Type) : Type := m (Action a).
 
 Definition runLoopeT {m A} (loop : LoopeT m A) : m (Action A) :=
   loop.
@@ -309,8 +315,6 @@ Arguments Monad m : assert.
 
 Print bind.
 
-Close Scope monad_scope.
-
 Global Program Instance loopeT_M  {m} `{Monad m} : Monad (LoopeT m) :=
   { return_ := @loopeT_pure m _;
     bind := @loopeT_bind m _  }.
@@ -340,61 +344,52 @@ Global Program Instance loopeT_M  {m} `{Monad m} : Monad (LoopeT m) :=
   unfold runLoopeT.
   unfold LoopeT in f.
   pose proof bind_left_unit.
-  generalize (H0 A a (Action B) f).
-  intros.
-  pose proof bind_right_unit.
-(*   rewrite H1 at 1. *)
-  pose proof bind_associativity.
-  pose proof actionM_obligation_2.
-  assert (bind (return_ a) f = bind (return_ (Atom a)) (fun _ => f a)).
-  + cbn.
-  rewrite equal_f .
-(*   case_eq (f (return_ a)). *)
-  rewrite H2 at 1.
-  refine 
-  case o ; auto.
-  apply f_equal.
-  apply functional_extensionality.
-  auto.
+  rewrite <- bind_left_unit.
+  reflexivity.
   Qed.
 
+  Next Obligation.
+  unfold loopeT_bind.
+  unfold runLoopeT.
+  rewrite <- bind_associativity.
+  f_equal.
+  apply functional_extensionality.
+  intros.
+  case_eq x ; auto ; intros; rewrite <- bind_left_unit; reflexivity.
+  Qed.
 
-(* Definition loopeT_bind  {A} (x : LoopeT m A) {B} (k : A -> LoopeT m B) : LoopeT m B :=
-    perf o <- runLoopeT x;
-    match o with
-      | Break => return_ Break
-      | Atom y => runLoopeT (k y)
-    end. *)
+(* Definition loopeT_liftT {m A} `{Monad m} (a : m A) : LoopeT m A.
+Proof.
+unfold LoopeT.
+refine (perf x <- a; return_ (Atom x)).
+Defined. *)
 
-(* Class Monad (m: Type -> Type) :=
-{ return_ : forall {A}, A -> m A;
-  bind: forall {A}, m A -> forall {B}, (A -> m B) -> m B;
-  bind_right_unit: forall A (a: m A), a = bind a return_;
-  bind_left_unit: forall A (a: A) B (f: A -> m B),
-             f a = bind (return_ a) f;
-  bind_associativity: forall A (ma: m A) B f C (g: B -> m C),
-                 bind ma (fun  x=> bind (f x) g) = bind (bind ma f) g
-}. *)
+(* liftT : forall {A}, m A -> t m A; *)
+Definition loopeT_liftT {m} `{Monad m} {A} (a : m A) : LoopeT m A :=
+  liftM (@Atom A) a.
 
-(* Notation "'perf' x '<-' m ';' e" := (bind m (fun x => e)) *)
-
-
-(*                         
-  Proof.
-  + intros.
-    unfold runLoopeT.
-    cbv.
-    case H.
-    intros.
-    generalize (bind_right_unit0 (Action A) a).
-    intros.
-    unfold LoopeT in *.
-    rewrite H0 at 1.
-    symmetry. *)
-    
-   
-(* Definition loopeT_liftT {m A} `{Monad m} (a : m A) : LoopeT m A :=
-  liftM (@Atom A) a. *)
+Global Program Instance LoopeT_T {m} `{Monad m} : MonadTrans (LoopeT):=
+  { liftT := @loopeT_liftT m _}.
+  Next Obligation.
+  unfold loopeT_liftT.
+  unfold loopeT_pure.
+  unfold liftM.
+  rewrite <- bind_left_unit.
+  reflexivity.
+  Qed.
+  
+  Next Obligation.
+  unfold loopeT_liftT.
+  unfold loopeT_bind.
+  unfold liftM.
+  unfold runLoopeT.
+  rewrite <- bind_associativity.
+  rewrite <- bind_associativity.
+  f_equal.
+  extensionality x.
+  rewrite <- bind_left_unit.
+  reflexivity.
+  Qed.
 
 Definition break {m A} `{Monad m} : LoopeT m A :=
   return_ Break.
@@ -402,7 +397,7 @@ Definition break {m A} `{Monad m} : LoopeT m A :=
 Fixpoint foreach2 {m} `{Monad m}(it min : nat) (body : nat -> LoopeT m unit) : m unit :=
   if (it <=? min) then return_ tt
   else match it with
-        | S it' => perf out <- (body it');
+        | S it' => perf out <- runLoopeT (body it');
                                 match out with
                                   | Break => return_ tt
                                   | _ => foreach2 it' min body
@@ -416,7 +411,8 @@ Fixpoint foreach2 {m} `{Monad m}(it min : nat) (body : nat -> LoopeT m unit) : m
   else [].
 Next Obligation. apply Zabs_nat_lt; auto with zarith. Qed. *)
 
-Program Fixpoint foreach3 (from to : Z) (body : Z -> LoopeT m unit) {measure (Z.abs_nat (to - from))} : m unit :=
+
+Program Fixpoint foreach3 {m} `{Monad m} (from to : Z) (body : Z -> LoopeT m unit) {measure (Z.abs_nat (to - from))} : m unit :=
   if Z_lt_dec from to
   then perf out <- runLoopeT (body from);
                                 match out with
@@ -427,6 +423,7 @@ Program Fixpoint foreach3 (from to : Z) (body : Z -> LoopeT m unit) {measure (Z.
 Next Obligation. 
 apply Zabs_nat_lt; auto with zarith. Qed.
 
+End monad_option.
 End monadic_loop2.
 
 Notation "'for' i '=' max 'to' min '{{' body }}" := (foreach max min (fun i => (loopT_liftT body))) (at level 60, i ident, min at level 60,
@@ -441,5 +438,5 @@ max at level 60, body at level 60, right associativity) : monad_scope.
 Notation "'for2_e' i '=' max 'to' min '{{' body }}" := (foreach2 min max (fun i => (body))) (at level 60, i ident, min at level 60,
 max at level 60, body at level 60, right associativity) : monad_scope.
 
-Notation "'for3' i '=' max 'to' min '{{' body }}" := (foreach2 min max (fun i => (body))) (at level 60, i ident, min at level 60,
+Notation "'for3' i '=' min 'to' max '{{' body }}" := (foreach3 min max (fun i => (loopeT_liftT body))) (at level 60, i ident, min at level 60,
 max at level 60, body at level 60, right associativity) : monad_scope.
